src/Iris/Algebra/HeapView.lean
@@ -475,16 +475,16 @@ end heapUpdates
 
 section heapViewFunctor
 
-open Iris.Std
+open Iris.Std PartialMap
 
 theorem heapR_map_eq [OFE A] [OFE B] [OFE A'] [OFE B'] [RFunctor T] (f : A' -n> A) (g : B -n> B')
     (n : Nat) (m : H (T A B)) (mv : H (DFrac F × T A B)) :
     HeapR F K (T A B) H n m mv →
     HeapR F K (T A' B') H n
-      ((Heap.mapO H (RFunctor.map f g).toHom).f m)
-      ((Heap.mapC H (Prod.mapC (CMRA.Hom.id (α := DFrac F))
+      ((mapO H (RFunctor.map f g).toHom).f m)
+      ((mapC H (Prod.mapC (CMRA.Hom.id (α := DFrac F))
       (RFunctor.map (F:=T) f g))).f mv) := by
-  simp [HeapR, Heap.mapC, Heap.mapO, Heap.map, CMRA.Hom.id, OFE.Hom.id, Prod.mapC, get?_bindAlter]
+  simp [HeapR, PartialMap.mapC, PartialMap.mapO, PartialMap.map, CMRA.Hom.id, OFE.Hom.id, Prod.mapC, get?_bindAlter]
   intros hr k a b
   rcases h : get? mv k with _ | ⟨a,b⟩ <;> simp
   rintro rfl rfl
@@ -515,40 +515,44 @@ abbrev HeapViewURF T [RFunctor T] : COFE.OFunctorPre :=
 instance {T} [RFunctor T] : URFunctor (HeapViewURF (F := F) (H := H) T) where
   map {A A'} {B B'} _ _ _ _ f g :=
     View.mapC
-      (Heap.mapO H (RFunctor.map f g).toHom)
-      (Heap.mapC H (Prod.mapC Hom.id (RFunctor.map f g)))
+      (PartialMap.mapO H (RFunctor.map f g).toHom)
+      (PartialMap.mapC H (Prod.mapC Hom.id (RFunctor.map f g)))
       (heapR_map_eq f g)
   map_ne.ne n _ _ Hx _ _ Hy mv := by
     apply View.map_ne
-    · refine fun _ => Heap.map_ne _ _ _ (RFunctor.map_ne.ne ?_ ?_) <;> simp_all
-    · refine fun _ => Heap.map_ne _ _ _ ?_
+    · refine fun _ => ?_
+      apply PartialMap.map_ne
+      exact RFunctor.map_ne.ne Hx Hy
+    · refine fun _ => ?_
+      apply PartialMap.map_ne _ _ _
       exact fun _ => Prod.map_ne (fun _ => rfl) (RFunctor.map_ne.ne Hx Hy)
   map_id x := by
     rw (config := { occs := .pos [2] }) [<- (View.map_id x)]
     apply View.map_ext
-    · exact (COFE.OFunctor.map_id (F := HeapOF H T))
+    · exact (COFE.OFunctor.map_id (F := PartialMapOF H T))
     · intro b
-      refine (Equiv.trans ?_ (Heap.map_id _ b))
-      refine equiv_dist.mpr (fun n => (Heap.map_ne _ (n := n) _ _ ?_))
+      refine (Equiv.trans ?_ (map_id _ b))
+      refine equiv_dist.mpr (fun n => ?_)
+      apply PartialMap.map_ne
       exact fun _ => ⟨rfl, Equiv.dist (RFunctor.map_id _)⟩
   map_comp f g f' g' x := by
     simp [View.mapC]
     rw [<- View.map_compose']
     apply View.map_ext
-    · apply (inferInstance : URFunctor (HeapOF H T)).map_comp
-    · simp [Prod.mapC, CMRA.Hom.id, Heap.mapC]
+    · apply (inferInstance : URFunctor (PartialMapOF H T)).map_comp
+    · simp [Prod.mapC, CMRA.Hom.id, PartialMap.mapC]
       intro
       symm
       apply OFE.Equiv.trans
-      exact (OFE.Equiv.symm (Heap.map_compose _ _ _ _))
-      apply Heap.map_ext
+      exact (OFE.Equiv.symm (PartialMap.map_compose _ _ _ _))
+      apply PartialMap.map_ext
       rw [Prod.map_comp_map]
       apply (fun _ => Prod.map_ext _ _) <;> simp
       exact (fun _ x => OFE.Equiv.symm (RFunctor.map_comp _ _ _ _ x))
 
 instance {T} [RFunctorContractive T] : URFunctorContractive (HeapViewURF (F := F) (H := H) T) where
   map_contractive.1 H _ := by
-    apply View.map_ne <;> intros <;> apply Heap.map_ne
+    apply View.map_ne <;> intros <;> apply PartialMap.map_ne
     · exact (RFunctorContractive.map_contractive.1 H)
     · exact (fun _ => Prod.map_ne (fun _ => rfl) (RFunctorContractive.map_contractive.1 H))
 
